okasaki/BankersDeque_proof.v
@@ -1,0 +1,126 @@
+Set Implicit Arguments.
+Require Import FuncTactics LibCore.
+Require Import DequeSig_ml DequeSig_proof.
+Require Import BankersDeque_ml.
+
+Definition C := 2.
+
+Lemma c_val : c = C.
+Proof. xgo~. Qed.
+
+
+Module BankersQueueSpec <: QueueSigSpec.
+
+(** instantiations *)
+
+Module Import Q <: MLDeque := MLBankersDeque.
+Import MLBankersDeque.
+
+(** invariant *)
+
+Definition inv (d:int) `{Rep a_ A} (q:deque a_) (Q:list A) :=
+  let '(lenf,f,lenr,r) := q in 
+     Forall2 rep (f ++ rev r) Q
+  /\ lenf = length f
+  /\ lenr = length r
+  /\ lenf <= C*lenr + 1 + d
+  /\ lenr <= C*lenf + 1 + d.
+
+Global Instance deque_rep `{Rep a_ A} : Rep (deque a_) (list A) :=
+  inv 0.
+
+(** automation *)
+
+Lemma c_val2 : c = 2.
+Proof. rewrite~ c_val. Qed.
+Hint Rewrite c_val2 : rew_maths.
+
+Hint Constructors Forall2.
+Hint Resolve Forall2_last.
+Hint Extern 1 (@rep (deque _) _ _ _ _) => simpl.
+Hint Unfold inv.
+
+Ltac auto_tilde ::= eauto with maths.
+
+Section Polymorphic.
+Variables (a_ A : Type) (RA:Rep a_ A).
+
+(** useful facts *)
+
+Lemma empty_from_len : forall f lenf lenr r Q,
+  rep (lenf, f, lenr, r) Q -> lenf + lenr = 0 -> Q = nil.
+Proof.
+  introv (H&LF&LR&CF&CR) L.  
+  rewrite~ (@length_zero_inv _ r) in H.
+  rewrite~ (@length_zero_inv _ f) in H.
+  inverts~ H.
+Qed.
+
+(** verification *)
+
+Lemma empty_spec : 
+  rep (@empty a_) (@nil A).
+Proof.
+  generalizes RA A. apply (empty_cf a_). xgo.
+  intros. simpl. rew_list~.
+Qed.
+
+Hint Extern 1 (RegisterSpec empty) => Provide empty_spec.
+
+Lemma is_empty_spec : 
+  RepTotal is_empty (Q;deque a_) >> bool_of (Q = nil).
+Proof.
+  xcf. intros (((lenf,f),lenr),r) Q RQ. xgo.
+  unfolds. extens. iff Z; fold_prop; subst.
+  apply~ empty_from_len.
+  intuit RQ. inverts H. destruct (nil_eq_app_rev_inv H5). subst~.
+Qed. 
+
+Hint Extern 1 (RegisterSpec is_empty) => Provide is_empty_spec.
+
+Lemma check_spec : 
+  Spec check (q:deque a_) |R>>
+    forall Q, inv 1 q Q ->
+    R (Q ; deque a_).
+Proof.
+  xcf. intros (((lenf,f),lenr),r) Q K. xgo.
+  destructs K. subst. simple~.
+  destructs K. simpl. rew_list~.
+Qed.
+
+Hint Extern 1 (RegisterSpec check) => Provide check_spec.
+
+Lemma snoc_spec : 
+  RepTotal snoc (Q;deque a_) (X;a_) >> (Q & X) ; deque a_.
+Proof.
+  xcf. intros (((lenf,f),lenr),r) x. introv (H&LF&LR&LE) RX.
+  xgo~; ximpl_nointros. unfolds. rew_list. rewrite~ <- app_assoc. 
+Qed.
+
+Hint Extern 1 (RegisterSpec snoc) => Provide snoc_spec.
+
+Lemma head_spec : 
+  RepSpec head (Q;deque a_) |R>>
+     Q <> (@nil A) -> R (is_head Q ;; a_).
+Proof.
+  xcf. intros (((lenf,f),lenr),r) Q RQ NE. xgo.
+  apply NE. apply~ empty_from_f.
+  intuit RQ. inverts* H.
+Qed.
+
+Hint Extern 1 (RegisterSpec head) => Provide head_spec.
+
+Lemma tail_spec :
+  RepSpec tail (Q;deque a_) |R>> 
+     Q <> nil -> R (is_tail Q ;; deque a_).
+Proof.
+  xcf. intros (((lenf,f),lenr),r) Q RQ NE. xmatch.
+  apply NE. apply~ empty_from_f.
+  intuit RQ. rew_list in *. inverts H. xapp~. ximpl~.
+Qed.
+
+Hint Extern 1 (RegisterSpec tail) => Provide tail_spec.
+
+End Polymorphic.
+
+End BankersQueueSpec.
