okasaki/DequeSig_proof.v
@@ -1,0 +1,50 @@
+Set Implicit Arguments.
+Require Import FuncTactics DequeSig_ml LibCore.
+
+Module Type QueueSigSpec.
+
+Declare Module Q : MLDeque.
+Import Q.
+
+Global Instance deque_rep : forall `{Rep a_ A},  
+  Rep (deque a_) (list A).
+
+Section Polymorphic.
+Variables (a_ A : Type) (RA:Rep a_ A).
+
+Parameter empty_spec : 
+  rep (@empty a_) (@nil A).
+
+Parameter is_empty_spec : 
+  RepTotal is_empty (Q;deque a_) >> bool_of (Q = nil).
+
+Parameter cons_spec : 
+  RepTotal cons (X;a_) (Q;deque a_) >> (X::Q) ; deque a_.
+
+Parameter head_spec : 
+  RepSpec head (Q;deque a_) |R>>
+     Q <> (@nil A) -> R (is_head Q ;; a_).
+
+Parameter tail_spec :
+  RepSpec tail (Q;deque a_) |R>> 
+     Q <> nil -> R (is_tail Q ;; deque a_).
+
+Parameter snoc_spec : 
+  RepTotal snoc (Q;deque a_) (X;a_) >> (Q&X) ; deque a_.
+
+Parameter last_spec : 
+  RepSpec last (Q;deque a_) |R>>
+     Q <> (@nil A) -> R (is_last Q ;; a_).
+
+Parameter init_spec :
+  RepSpec init (Q;deque a_) |R>> 
+     Q <> nil -> R (is_init Q ;; deque a_).
+
+End Polymorphic.
+
+End QueueSigSpec.
+
+
+
+
+
